\subsubsection{Divergence of a product}
\begin{equation}
	\vec{\nabla} \cdot \left( f \vec{A} \right) = f \vec{\nabla} \cdot \vec{A} + \vec{A} \cdot \vec{\nabla} f
\end{equation}

\subsubsection{Curl of a gradient}
\begin{equation}
	\vec{\nabla} \wedge \vec{\nabla} f = 0
\end{equation}

\subsubsection{Divergence of a curl}
\begin{equation}
	\vec{\nabla} \cdot \left(\vec{\nabla} \wedge \vec{A}\right) = 0
\end{equation}

\subsubsection{Curl of a curl}
\begin{equation}
	\vec{\nabla} \wedge \left( \vec{\nabla} \wedge \vec{A} \right) = \vec{\nabla} \left( \vec{\nabla} \cdot \vec{A} \right) - \Delta \vec{A}
\end{equation}

\subsubsection{Divergence of a cross product}
\begin{equation}
	\vec{\nabla} \cdot \left( \vec{A} \wedge \vec{B} \right) = \vec{B} \cdot \left( \vec{\nabla} \wedge \vec{A} \right) - \vec{A} \cdot \left( \vec{\nabla} \wedge \vec{B} \right)
\end{equation}

\subsubsection{Curl of a cross product}
\begin{equation}
	\vec{\nabla} \wedge \left( \vec{A} \wedge \vec{B} \right) =  \left(\vec{B} \cdot \vec{\nabla} \right) \vec{A} - \left(\vec{A} \cdot \vec{\nabla} \right) \vec{B}  + \vec{A} \left( \vec{\nabla} \cdot \vec{B} \right) - \vec{B} \left( \vec{\nabla} \cdot \vec{A} \right)
\end{equation}